named_api/Functoriality/functoriality.v
@@ -23,7 +23,7 @@ Section Functoriality.
   Context (binder : aname -> term -> term -> term).
 
   (* 1. Add uparams + uparams_bis + function A -> A_bis *)
-  (* returns uparams, strpos_uparams, uparams_bis, functions *)
+  (* returns uparams, uparams_bis, functions *)
   Definition closure_uparams_func : state -> kername ->
       (state -> keys -> keys -> keys -> term) -> term :=
     fun s kname =>
@@ -134,16 +134,16 @@ Fixpoint add_param (s : state) (strpos : list bool) (l : list term) (rc : list t
 end.
 
 Fixpoint make_func_call (s : state) (key_arg : key) (ty : term) {struct ty} : term :=
-  match view_uparams_args s kname Ep [] key_uparams ty with
-  | UPArgIsUparam pos_uparams loc iargs =>
+  match view_uparams_args s kname Ep [] key_uparams strpos_uparams ty with
+  | SPArgIsSPUparam pos_uparams loc iargs =>
       let* s _ key_locals _ := closure_context_sep tLambda s (Some "locals") loc in
       mkApp (geti_term s key_funcs pos_uparams)
             (mkApps (get_term s key_arg) (get_terms s key_locals))
-  | UPArgIsInd pos_indb loc local_nuparams local_indices =>
+  | SPArgIsInd pos_indb loc local_nuparams local_indices =>
       let* s _ key_locals _ := closure_context_sep tLambda s (Some "locals") loc in
       mkApp (mkApps (geti_term s key_fixs pos_indb) (local_nuparams ++ local_indices))
             (mkApps (get_term  s key_arg) (get_terms s key_locals))
-  | UPArgIsNested xp pos_indb loc local_uparams local_nuparams_indices =>
+  | SPArgIsNested xp pos_indb loc local_uparams local_nuparams_indices =>
       let compute_nested_rc (x : term) (s s : state) : term :=
         let* s key_farg := mk_tLambda s (Some "rec_arg") (mkBindAnn nAnon Relevant) x in
         make_func_call s key_farg (lift0 1 x)
@@ -153,9 +153,9 @@ Fixpoint make_func_call (s : state) (key_arg : key) (ty : term) {struct ty} : te
       let ltm := add_param s xp.(ep_strpos_uparams) local_uparams rec_call in
           mkApp (mkApps (tConst xp.(ep_func_kname) []) (ltm ++ local_nuparams_indices))
                 (mkApps (get_term  s key_arg) (get_terms s key_locals))
-  | UPArgIsFree loc m iargs =>
+  | SPArgIsFree loc m iargs =>
       let* s _ key_locals _ := closure_context_sep tLambda s (Some "locals") loc in
-      mkApps (get_term  s key_arg) (get_terms s key_locals)
+      mkApps (get_term s key_arg) (get_terms s key_locals)
   end.
 
 Definition compute_args_fix : keys -> list term :=
