named_api/UnitTests/unit_tests.v
@@ -250,15 +250,15 @@ End TestFunctions.
 Definition generate {A} Ep : A -> _ := generate_options true false StopTests
                                         false false false false false false false Ep. *)
 
-Definition print_rec := print_rec_options false false false StopTests.
+(* Definition print_rec := print_rec_options false false false StopTests.
 Definition generate {A} Ep : A -> _ := generate_options false true StopTests
-                                        false false false false false false false Ep.
+                                        false false false false false false false Ep. *)
 
     (* ### Debug Recursor ### *)
 
-(* Definition print_rec := print_rec_options true false false TestRecType.
+Definition print_rec := print_rec_options true false false TestRecType.
 Definition generate {A} Ep : A -> _ := generate_options false false TestRecType
-                                        true false false false false false false Ep. *)
+                                        true false false false false false false Ep.
 
 (* Definition print_rec := print_rec_options false true false TestRecTerm.
 Definition generate {A} Ep : A -> _ := generate_options false false TestRecTerm
